a bit of progress

LangDesignImplVerif/IntArithVars.thy
@@ -12,131 +12,175 @@ type_synonym input = "int list"
 
 type_synonym env = "name \<rightharpoonup> int"
 
-fun E :: "exp \<Rightarrow> env \<Rightarrow> input \<Rightarrow> int option \<times> input" where
-  "E (EInt n) \<rho> stdin = (Some n,stdin)" |
-  "E (ERead) \<rho> stdin = (case stdin of [] \<Rightarrow> (None, [])
-                        | Cons n stdin' \<Rightarrow> (Some n, stdin'))" |
-  "E (ENeg e) \<rho> stdin = (case E e \<rho> stdin of (None,stdin') \<Rightarrow> (None,stdin')
-                        | (Some n,stdin') \<Rightarrow> (Some (- n), stdin'))" |
+fun E :: "exp \<Rightarrow> env \<Rightarrow> input \<Rightarrow> (int \<times> input) option" where
+  "E (EInt n) \<rho> stdin = Some (n,stdin)" |
+  "E (ERead) \<rho> stdin = (case stdin of [] \<Rightarrow> None
+                        | Cons n stdin' \<Rightarrow> Some (n, stdin'))" |
+  "E (ENeg e) \<rho> stdin = (case E e \<rho> stdin of None \<Rightarrow> None
+                        | Some (n,stdin') \<Rightarrow> Some (- n, stdin'))" |
   "E (EAdd e1 e2) \<rho> stdin =
-     (case E e1 \<rho> stdin of (None,stdin') \<Rightarrow> (None,stdin')
-      | (Some n1,stdin') \<Rightarrow> 
+     (case E e1 \<rho> stdin of None \<Rightarrow> None
+      | Some (n1,stdin') \<Rightarrow> 
         (case E e2 \<rho> stdin' of
-          (None,stdin'') \<Rightarrow> (None,stdin'')
-        | (Some n2,stdin'') \<Rightarrow> (Some (n1 + n2), stdin'')))" |
-  "E (EVar x) \<rho> stdin = (\<rho> x, stdin)" |
+          None \<Rightarrow> None
+        | Some (n2, stdin'') \<Rightarrow> Some (n1 + n2, stdin'')))" |
+  "E (EVar x) \<rho> stdin = (case \<rho> x of None \<Rightarrow> None | Some n \<Rightarrow> Some (n, stdin))" |
   "E (ELet x e1 e2) \<rho> stdin =
-     (case E e1 \<rho> stdin of (None,stdin') \<Rightarrow> (None,stdin')
-      | (Some n,stdin') \<Rightarrow> E e2 (\<rho>(x\<mapsto>n)) stdin')"
-  
+     (case E e1 \<rho> stdin of None \<Rightarrow> None
+      | Some (n,stdin') \<Rightarrow> E e2 (\<rho>(x\<mapsto>n)) stdin')"
+
 section "Intermediate Language in A-normal form"
   
 datatype atom = AInt int | AVar name
-datatype fexp = Atom atom | FRead | FNeg atom | FAdd atom atom
-datatype stmt = SLet name fexp | SReturn fexp
+datatype fexp = Atom atom | FNeg atom | FAdd atom atom
+datatype stmt = Assign name fexp | Read name 
+type_synonym block = "stmt list \<times> fexp"
 
 fun A :: "atom \<Rightarrow> env \<Rightarrow> int option" where
   "A (AInt n) \<rho> = Some n" |
   "A (AVar x) \<rho> = \<rho> x" 
   
-fun F :: "fexp \<Rightarrow> env \<Rightarrow> input \<Rightarrow> int option \<times> input" where
-  "F (Atom a) \<rho> stdin = (A a \<rho>, stdin)" |
-  "F (FRead) \<rho> stdin = (case stdin of [] \<Rightarrow> (None, [])
-                        | Cons n stdin' \<Rightarrow> (Some n, stdin'))" |
-  "F (FNeg e) \<rho> stdin = (case A e \<rho>  of None \<Rightarrow> (None,stdin)
-                        | Some n \<Rightarrow> (Some (- n),stdin))" |
-  "F (FAdd e1 e2) \<rho> stdin =
-     (case A e1 \<rho> of None \<Rightarrow> (None,stdin)
+fun F :: "fexp \<Rightarrow> env \<Rightarrow> int option" where
+  "F (Atom a) \<rho> = A a \<rho>" |
+  "F (FNeg e) \<rho> = (case A e \<rho>  of None \<Rightarrow> None
+                        | Some n \<Rightarrow> Some (- n))" |
+  "F (FAdd e1 e2) \<rho> =
+     (case A e1 \<rho> of None \<Rightarrow> None
       | Some n1 \<Rightarrow> 
         (case A e2 \<rho> of
-          None \<Rightarrow> (None,stdin)
-        | Some n2 \<Rightarrow> (Some (n1 + n2), stdin)))"
+          None \<Rightarrow> None
+        | Some n2 \<Rightarrow> Some (n1 + n2)))"
 
-fun S :: "stmt \<Rightarrow> env \<Rightarrow> input \<Rightarrow> (int option \<times> input) + (env \<times> input)" where
-  "S (SReturn e) \<rho> i = Inl (F e \<rho> i)" |
-  "S (SLet x e) \<rho> i =
-     (case F e \<rho> i of (None,i') \<Rightarrow> Inl (None,i')
-      | (Some n, i') \<Rightarrow> Inr (\<rho>(x\<mapsto>n), i'))"
+type_synonym state = "env \<times> input"
+type_synonym state_xfr = "state \<Rightarrow> state option"
 
-fun Ss :: "stmt list \<Rightarrow> env \<Rightarrow> input \<Rightarrow> (int option \<times> input) + (env \<times> input)" where
-  "Ss [] \<rho> i = Inr (\<rho>,i)" |
-  "Ss (s#ss) \<rho> i =
-     (case S s \<rho> i of
-       Inl r \<Rightarrow> Inl r
-     | Inr (\<rho>',i') \<Rightarrow> Ss ss \<rho>' i')"  
+fun S :: "stmt \<Rightarrow> state_xfr" where
+  "S (Assign x e) (\<rho>, i) =
+     (case F e \<rho> of None \<Rightarrow> None
+      | Some n \<Rightarrow> Some (\<rho>(x\<mapsto>n), i))" |
+  "S (Read x) (\<rho>, i) = (case i of [] \<Rightarrow> None
+                     | Cons n i' \<Rightarrow> Some (\<rho>(x\<mapsto>n), i'))"
 
-fun P :: "stmt list \<Rightarrow> env \<Rightarrow> input \<Rightarrow> int option \<times> input" where
-  "P ss \<rho> i = 
-     (case Ss ss \<rho> i of
-       Inl r \<Rightarrow> r
-     | Inr (\<rho>',i') \<Rightarrow> (None, i'))"   
+definition seq :: "state_xfr \<Rightarrow> state_xfr \<Rightarrow> state_xfr" where
+  "seq f1 f2 s \<equiv> (case f1 s of None \<Rightarrow> None | Some s' \<Rightarrow> f2 s')"
+
+fun ret :: "state_xfr" where
+  "ret \<sigma> = Some \<sigma>"
   
+fun Ss :: "stmt list \<Rightarrow> state_xfr" where
+  "Ss [] = ret" |
+  "Ss (s#ss) = seq (S s) (Ss ss)"
+
+fun B :: "block \<Rightarrow> state \<Rightarrow> (int \<times> input) option" where
+  "B (ss,e) (\<rho>, i) = 
+     (case Ss ss (\<rho>, i) of
+       None \<Rightarrow> None
+     | Some (\<rho>',i') \<Rightarrow> 
+       (case F e \<rho>' of None \<Rightarrow> None | Some n \<Rightarrow> Some (n, i')))"   
+
+lemma seq_some[simp]: "seq Some f = f"
+  unfolding seq_def apply (rule ext) apply auto done
+
+lemma seq_assoc[simp]: "seq (seq f1 f2) f3 = seq f1 (seq f2 f3)" 
+  unfolding seq_def apply (rule ext) apply auto apply (case_tac "f1 (a,b)") apply auto done
+
+lemma Ss_append_seq[simp]: "Ss (ss1@ss2) = seq (Ss ss1) (Ss ss2)"
+  by (induction ss1) auto
+    
+lemma Ss_none_seq[simp]: "Ss ss1 \<sigma> = None \<Longrightarrow> seq (Ss ss1) (Ss ss2) \<sigma> = None"
+  by (simp add: seq_def)
+    
+lemma Ss_some_seq[simp]: "Ss ss1 \<sigma> = Some \<sigma>' \<Longrightarrow> seq (Ss ss1) (Ss ss2) \<sigma> = (Ss ss2) \<sigma>'"
+  by (simp add: seq_def)
+
 section "Compilation Pass: Flattening"
 
-fun atomize :: "fexp \<Rightarrow> nat \<Rightarrow> nat \<times> atom \<times> (stmt list)" where
-  "atomize (Atom a) k = (k, a, [])" |
-  "atomize f k = (Suc k, AVar k, [SLet k f])"
-  
-fun flatten :: "exp \<Rightarrow> nat \<Rightarrow> nat \<times> fexp \<times> (stmt list)" where
-  "flatten (EInt n) k = (k, Atom (AInt n), [])" |
-  "flatten (ERead) k = (k+1, Atom (AVar k), [SLet k FRead])" |
-  "flatten (ENeg e) k = 
-    (let (k1,e',ss1) = flatten e k in
-     let (k2,a,ss2) = atomize e' k1 in
-     (k2, FNeg a, ss1@ ss2))" |
-  "flatten (EAdd e1 e2) k =
-    (let (k1,e1',ss1) = flatten e1 k in
-     let (k2,e2',ss2) = flatten e2 k1 in
-     let (k3,a1,c3) = atomize e1' k2 in
-     let (k4,a2,c4) = atomize e2' k3 in
-     (k4, FAdd a1 a2, ss1 @ ss2 @ c3 @ c4))" |
-  "flatten (EVar x) k = (k, Atom (AVar x), [])" |
-  "flatten (ELet x e1 e2) k = 
-    (let (k1,e1',ss1) = flatten e1 k in
-     let (k2,e2',ss2) = flatten e2 k1 in
-     (k2, e2', ss1 @ (SLet x e1') # ss2))"
+fun atomize :: "fexp \<Rightarrow> nat \<Rightarrow> nat \<times> (stmt list) \<times> atom" where
+  "atomize (Atom a) k = (k, [], a)" |
+  "atomize f k = (Suc k, [Assign k f], AVar k)"
 
-fun flatten_program :: "exp \<Rightarrow> stmt list" where
-  "flatten_program e = (let (k,e',ss) = flatten e 0 in ss @ [SReturn e'])" 
-  
+fun flatten :: "exp \<Rightarrow> nat \<Rightarrow> nat \<times> block" where
+  "flatten (EInt n) k = (k, [], Atom (AInt n))" |
+  "flatten (ERead) k = (k+1, [Read k], Atom (AVar k))" |
+  "flatten (ENeg e) k = 
+    (let (k1,ss1,e') = flatten e k in
+     let (k2,ss2,a) = atomize e' k1 in
+     (k2, ss1@ ss2, FNeg a))" |
+  "flatten (EAdd e1 e2) k =
+    (let (k1,ss1,e1') = flatten e1 k in
+     let (k2,ss2,e2') = flatten e2 k1 in
+     let (k3,c3,a1) = atomize e1' k2 in
+     let (k4,c4,a2) = atomize e2' k3 in
+     (k4, ss1 @ ss2 @ c3 @ c4, FAdd a1 a2))" |
+  "flatten (EVar x) k = (k, [], Atom (AVar x))" |
+  "flatten (ELet x e1 e2) k = 
+    (let (k1,ss1,e1') = flatten e1 k in
+     let (k2,ss2,e2') = flatten e2 k1 in
+     (k2, ss1 @ (Assign x e1') # ss2, e2'))"
+
+fun flatten_program :: "exp \<Rightarrow> block" where
+  "flatten_program e = (let (k,ss,e') = flatten e 0 in (ss, e'))" 
+
 value "flatten_program (ENeg (EAdd (EInt 1) (ENeg (EInt 2))))"
   
 section "Correctness of Flattening"
-  
-lemma atomize_correct: "atomize e k = (k', a, ss) \<Longrightarrow> Ss [SReturn e] = Ss (ss @ [SReturn (Atom a)])"
+
+lemma atomize_correct: "atomize e k = (k', ss, a) \<Longrightarrow> B ([], e) = B (ss, Atom a)"
   apply (cases e)
   apply force
-    apply simp apply clarify apply (rule ext) apply (rule ext) apply simp
-    apply (case_tac xa) apply force apply force
-  apply simp apply (rule ext) apply (rule ext) apply simp apply clarify apply (case_tac "A x3 x")
-    apply force apply force
-  apply simp apply (rule ext) apply (rule ext) apply simp apply (case_tac "A x41 x") apply force
-  apply simp apply (case_tac "A x42 x") apply auto 
+  apply simp apply clarify apply (rule ext) apply (case_tac x) apply simp
+    apply (case_tac "A x2 aa") apply auto
+    apply (simp add: seq_def)
+    apply (simp add: seq_def)
+  apply (rule ext) apply (case_tac x) apply (simp add: seq_def) 
+    apply (case_tac "A x31 aa") apply (auto simp: seq_def)
+    apply (case_tac "A x32 aa") apply (auto simp: seq_def)
   done
   
-lemma S_append_cong2[cong]: "\<lbrakk> Ss ss2 = Ss ss2' \<rbrakk> \<Longrightarrow>
-    Ss (ss1 @ ss2) \<rho> i = Ss (ss1 @ ss2') \<rho> i"
-  apply (induction ss1 arbitrary: \<rho> i)
-  apply force
-  apply simp apply (case_tac "S a \<rho> i") apply force apply force
-  done
-    
-lemma flatten_correct: "flatten e k = (k', e', ss) \<Longrightarrow> E e \<rho> i = P (ss @ [SReturn e']) \<rho> i"
+lemma flatten_correct: "flatten e k = (k', ss, e') \<Longrightarrow> E e \<rho> i = B (ss, e') (\<rho>, i)"
 proof (induction e arbitrary: k k' e' \<rho> i ss)
   case (EInt n)
-  have 1: "E (EInt n) \<rho> i = (Some n,i)" by simp
-  have 2: "flatten (EInt n) k = (k, Atom (AInt n), [])" by simp
-  have 3: "P ([] @ [SReturn (Atom (AInt n))]) \<rho> i = (Some n, i)" by simp
+  have 1: "E (EInt n) \<rho> i = Some (n,i)" by simp
+  have 2: "flatten (EInt n) k = (k, [], Atom (AInt n))" by simp
+  have 3: "B ([], Atom (AInt n)) (\<rho>, i) = Some (n, i)" by simp
   from EInt 1 2 3 show ?case by simp
 next
   case ERead
-  have 2: "flatten ERead k = (Suc k, Atom (AVar k), [SLet k FRead])" by simp
-  have 3: "E ERead \<rho> i = P ([SLet k FRead] @ [SReturn (Atom (AVar k))]) \<rho> i" by (cases i) auto 
+  have 2: "flatten ERead k = (Suc k, [Read k], Atom (AVar k))" by simp
+  have 3: "E ERead \<rho> i = B ([Read k], Atom (AVar k)) (\<rho>, i)" by (cases i) (auto simp: seq_def) 
   from ERead 2 3 show ?case by simp
 next
-  case (ENeg e)
-    
-  then show ?case sorry
+  case (ENeg e k k' e' \<rho> i ss)
+  obtain k1 e1 ss1 where fe: "flatten e k = (k1,ss1,e1)" by (case_tac "flatten e k") auto
+  obtain k2 a ss2 where ae1: "atomize e1 k1 = (k2,ss2,a)" by (case_tac "atomize e1 k1") auto
+  from fe ae1 ENeg have fne: "flatten (ENeg e) k = (k2, ss1@ss2, FNeg a)" by simp
+  from fne ENeg have ss: "ss = ss1 @ ss2" by simp
+  from fne ENeg have ep: "e' = FNeg a" by simp
+  from fe ENeg have IH: "E e \<rho> i = B (ss1, e1) (\<rho>, i)" by blast
+  from ae1 have 1: "B ([], e1) = B (ss2, Atom a)" using atomize_correct[of e1 k1] by blast
+  
+  from 1 have 2: "B (ss1 @ [], e1) (\<rho>, i) = B (ss1 @ ss2, Atom a) (\<rho>, i)"
+    apply simp apply (case_tac "Ss ss1 (\<rho>,i)") apply auto
+    apply (case_tac "F e1 aa") apply auto
+    apply (case_tac "Ss ss2 (aa,b)") apply auto
+     prefer 2 apply (case_tac "Ss ss2 (aa,b)") apply auto
+      sorry
+      
+  from IH 2 have 3: "E e \<rho> i = B (ss1 @ ss2, Atom a) (\<rho>, i)" by simp
+  have "E e \<rho> i = None \<or> (\<exists> n i'. E e \<rho> i = Some (n, i'))" by (case_tac "E e \<rho> i") auto
+  from this have 4: "E (ENeg e) \<rho> i = B (ss1 @ ss2, FNeg a) (\<rho>, i)"
+  proof
+    assume Ee: "E e \<rho> i = None"
+    from Ee 3 show ?thesis
+      apply (case_tac "seq (Ss ss1) (Ss ss2) (\<rho>,i)") apply force
+      apply (case_tac aa) apply (case_tac "A a aaa") apply auto done      
+  next assume "\<exists> n i'. E e \<rho> i = Some (n, i')"
+    from this obtain n i' where Ee: "E e \<rho> i = Some (n,i')" by blast
+    from Ee 3 show ?thesis apply simp
+      apply (case_tac "seq (Ss ss1) (Ss ss2) (\<rho>,i)") apply force apply auto
+      apply (case_tac "A a aa") apply auto done      
+  qed
+  from 4 ss ep show ?case by blast      
 next
   case (EAdd e1 e2)
   then show ?case sorry
@@ -147,38 +191,7 @@ next
   case (ELet x1a e1 e2)
   then show ?case sorry
 qed
-  
-  apply force
-  apply simp apply clarify apply (case_tac i) apply simp apply clarify apply simp
-       apply (subgoal_tac "[SLet k FRead] @ [SReturn (Atom (AVar k))] = [SLet k FRead,SReturn (Atom (AVar k))]")
-       prefer 2 apply force apply subst
-  prefer 3 apply force 
-proof -
-  fix e k k' e' \<rho> i ss
-  assume IH: "\<And>k k' e' \<rho> i ss. flatten e k = (k', e', ss) \<Longrightarrow> E e \<rho> i = S (ss @ [SReturn e']) \<rho> i"
-    and fl: "flatten (ENeg e) k = (k', e', ss)" 
-  obtain k1 e'' ss1 where fe: "flatten e k = (k1,e'',ss1)" apply (case_tac "flatten e k") by auto
-  obtain k2 a ss2 where aep: "atomize e'' k1 = (k2,a,ss2)" apply (case_tac "atomize e'' k1") by auto    
-  from fl fe aep have kp: "k' = k2" by simp
-  from fl fe aep have ep: "e' = FNeg a" by auto 
-  from fl fe aep have ss: "ss = ss1 @ ss2" by auto 
-  from IH fe have Ee_Sf: "E e \<rho> i = S (ss1 @ [SReturn e'']) \<rho> i" by blast    
-  from aep have 2: "S [SReturn e''] = S (ss2 @ [SReturn (Atom a)])" by (rule atomize_correct)
-  from Ee_Sf 2 have 3: "E e \<rho> i = S (ss1 @ ss2 @ [SReturn (Atom a)]) \<rho> i" apply simp
-      
-  from ep c show "E (ENeg e) \<rho> stdin = S (c (SReturn e'')) \<rho> stdin"
-  proof clarify
-    
-    show "E (ENeg e) \<rho> stdin = S (c1 (c2 (SReturn (FNeg a)))) \<rho> stdin" sorry
-     
-  qed
-next
-  fix e1 e2 x xa k k' e' c
-  show " E (EAdd e1 e2) x xa = S (c (SReturn e')) x xa" sorry
-next
-  fix x1a e1 e2 x xa k k' e' c
-  show "E (ELet x1a e1 e2) x xa = S (c (SReturn e')) x xa" sorry
-qed
+
   
 end
   
